src/SDK/MessageHeader/MessageHeader.dfy
@@ -15,57 +15,26 @@ module MessageHeader {
   import D = Deserialize
   import S = Serialize
 
-  /*
-   * Definition of the message header, i.e., the header body and the header authentication
-   */
-  class Header {
-    var body: Option<Definitions.HeaderBody>
-    var auth: Option<Definitions.HeaderAuthentication>
+  method Deserialize(is: Streams.StringReader) returns (res: Result<Definitions.Header>)
+    requires is.Valid()
+    modifies is
+    ensures is.Valid()
+    ensures match res
+      case Success(header) => Validity.ValidHeader(header)
+      case Failure(_) => true
+  {
+    var body :- D.DeserializeHeaderBody(is);
+    var auth :- D.DeserializeHeaderAuthentication(is, body.algorithmSuiteID);
+    return Success(Definitions.Header(body, auth));
+  }
 
-    constructor () {
-      body, auth := None, None;
-    }
-
-    method Deserialize(is: Streams.StringReader)
-      requires is.Valid()
-      requires body.None? || auth.None?
-      modifies is, `body, `auth
-      ensures body.Some? && auth.Some? ==> Validity.ValidHeaderBody(body.get)
-      ensures body.Some? && auth.Some? ==> Validity.ValidHeaderAuthentication(auth.get, body.get.algorithmSuiteID)
-      // TODO: is this the right decision?
-      ensures body.Some? <==> auth.Some?
-      ensures body.None? <==> auth.None? // redundant
-      ensures is.Valid()
-    {
-      var res := D.DeserializeHeaderBody(is);
-      match res {
-        case Success(body_) =>
-          assert body_.algorithmSuiteID in AlgorithmSuite.Suite.Keys; // nfv
-          var res := D.DeserializeHeaderAuthentication(is, body_.algorithmSuiteID);
-          match res {
-            case Success(auth_) =>
-              body, auth := Some(body_), Some(auth_);
-              assert Validity.ValidHeaderBody(body.get);
-            case Failure(e) =>
-              print "Could not deserialize message header: " + e + "\n";
-              body, auth := None, None;
-              return;
-          }
-        case Failure(e) =>
-          print "Could not deserialize message header: " + e + "\n";
-          body, auth := None, None;
-          return;
-      }
-    }
-
-    method Serialize(os: Streams.StringWriter) returns (ret: Result<nat>)
-      requires os.Valid()
-      requires body.Some?
-      requires Validity.ValidHeaderBody(body.get)
-      modifies os.Repr
-      ensures os.Valid()
-    {
-      ret := S.SerializeHeaderBody(os, body.get);
-    }
+  method Serialize(os: Streams.StringWriter, header: Definitions.Header) returns (ret: Result<nat>)
+    requires os.Valid() && Validity.ValidHeader(header)
+    modifies os.Repr
+    ensures os.Valid()
+  {
+    var m :- S.SerializeHeaderBody(os, header.body);
+    var n :- S.SerializeHeaderAuthentication(os, header.auth, header.body.algorithmSuiteID);
+    return Success(m + n);
   }
 }
